% $Id$

\subsection{Rings: Two associative operations}

\begin{definition}[Constructive Ring]\label{defring}
A non-trivial
{\em constructive ring\/} is a tuple \struct{S,0,1,+,-,*,=,\noto}
with \struct{S,0,+,-,=,\noto} a
constructive group and \struct{S,1,*,=,\noto} a
constructive monoid such that 
\begin{enumerate}
\item Non-triviality: $1\noto 0$.
\item $+$ distributes over $*$:\quad $\forall x,y,z[x*(y+z) = (x*y)+(x*z)]$.
\end{enumerate}
\end{definition}

\begin{notation}
When dealing with rings we replace the operation $*$ by juxtaposition,
writing $xy$ for $x*y$.
\end{notation}


\begin{lemma}\label{lemring}For all $x, y$:
  \begin{eqnarray*}
    x   0 &=& 0,\\
    x   (- y) &=& -(x y).
  \end{eqnarray*}
\end{lemma}

\begin{proof}
The first by cancellation: $x0=x(0+0)=x0+x0$. The second (using the
first) by uniqueness of inverses \ref{lemuninv}. \qed
\end{proof}

\begin{lemma}\label{lemHeyt}
For all $x,y$,
\begin{eqnarray*}
x  y \noto 0 &\implies& x\noto 0 \wedge y\noto 0.
\end{eqnarray*}
\end{lemma}
\begin{proof}
Suppose $x y \noto 0$. As $*$ is strongly extensional, we know 
$x y \noto x 0\implies y\noto 0$ and $x y \noto 0 y \implies x\noto 0$.
\qed
\end{proof}

